---
layout: post
title: I don't understand the Strong Law of Large Numbers
published: true
comments: true
---

I've been reading the article [An Elementary Proof of the Strong Law of Large Numbers](https://link.springer.com/article/10.1007/BF01013465)
since it's closely related to a result that I used in my [RNN theory](https://arxiv.org/abs/2308.12075).
I thought, once I understand it, I can refine my proof. However, I don't understand it. Yet :)

As I understand more I will update this post. For now, I will just write down my thoughts. This is the first page, and
the blue letters indicate the inequalities I will prove in more detail.

![slln1](/images/EPSLLN.png)

So, A is simply Chebyshev's inequality, B only needs to assume indipendence, and C is the first part that I found
tricky. Possibly obvious for a mathematician but not for me. First I wasn't sure about how I could change the summation
order, so, this is what I did

$$
\begin{align}
    \sum_{j=1}^{\infty}\sum_{i=1}^{\alpha^j} f(i)g(j)
    =&\sum_{j=1}^{\infty}\sum_{i=1}^{\infty} f(i)g(j)H(\alpha^j \geq i )\\
    =&\sum_{i=1}^{\infty}\sum_{j=1}^{\infty} f(i)g(j)H(\alpha^j \geq i )\\
    =&\sum_{i=1}^{\infty}\sum_{j=1}^{\infty} f(i)g(j)H(j \geq \log_\alpha i )\\
    =&\sum_{i=1}^{\infty}\sum_{j=\log_\alpha i}^{\infty} f(i)g(j)\\
\end{align}
$$

where $H$ is the Heaviside step function. Then I apply it to the sum in C, and I get

$$
\begin{align}
    \sum_{n=1}^{\infty}\frac{1}{\alpha^{2n}}\sum_{i=1}^{\alpha^n}f(i)=& \sum_{i=1}^{\infty}f(i)\sum_{n=\log_\alpha i}^{\infty}\frac{1}{\alpha^{2n}}\\
    =& \sum_{i=1}^{\infty}f(i)\Big(\sum_{n=1}^{\infty}\frac{1}{\alpha^{2n}}-\sum_{n=1}^{\log_\alpha i - 1}\frac{1}{\alpha^{2n}}\Big)\\
    =& \sum_{i=1}^{\infty}f(i)\Big(\frac{1}{1-r}-\frac{1-r^{\log_\alpha i}}{1-r}\Big) && \text{with } r=\alpha^{-2}\\
    =& \sum_{i=1}^{\infty}f(i)\frac{r^{\log_\alpha i}}{1-r} \\
    =& \sum_{i=1}^{\infty}\frac{1}{i^2}f(i)\frac{1}{1-r} \\
    =& \sum_{i=1}^{\infty}\frac{1}{i^2}f(i)\frac{\alpha^2}{\alpha^2-1} \\
    =& \frac{\alpha^2}{\alpha^2-1}\sum_{i=1}^{\infty}\frac{1}{i^2}f(i) \\
\end{align}
$$

Pretty cool eh? There might be some mistakes, but I think easy to fix. Also you need that $Var X \leq \E X^2$, which is
always true given that $Var X = \E X^2 - (\E X)^2$. I understand actually until equation 6 in this article, but
I want to finish other stuff so, enough for today!

Soon more. Enjoy!

{% if page.comments %} 



<div id="disqus_thread"></div>
<script>

/**
*  RECOMMENDED CONFIGURATION VARIABLES: EDIT AND UNCOMMENT THE SECTION BELOW TO INSERT DYNAMIC VALUES FROM YOUR PLATFORM OR CMS.
*  LEARN WHY DEFINING THESE VARIABLES IS IMPORTANT: https://disqus.com/admin/universalcode/#configuration-variables*/
/*
var disqus_config = function () {
this.page.url = PAGE_URL;  // Replace PAGE_URL with your page's canonical URL variable
this.page.identifier = PAGE_IDENTIFIER; // Replace PAGE_IDENTIFIER with your page's unique identifier variable
};
*/
(function() { // DON'T EDIT BELOW THIS LINE
var d = document, s = d.createElement('script');
s.src = 'https://https-lucehe-github-io.disqus.com/embed.js';
s.setAttribute('data-timestamp', +new Date());
(d.head || d.body).appendChild(s);
})();
</script>
<noscript>Please enable JavaScript to view the <a href="https://disqus.com/?ref_noscript">comments powered by Disqus.</a></noscript>



{% endif %}
